cil

proofs/compiler/cil.v
@@ -1,3 +1,6 @@
+From elpi.apps Require Import derive.std.
+From HB Require Import structures.
+
 From mathcomp Require Import
   ssreflect
   ssrbool
@@ -53,33 +56,32 @@ Section CIL.
 
 Class OracleSystem :=
   {
-    Mo : Type;
-    No : choiceType;
-    In : No -> choiceType;
-    Out : No -> choiceType;
-    Oo : forall (o : No), In o -> Mo -> itree Rnd (Out o * Mo);
-    orac_init_mem : Mo;
-    oI : No;
-    oI_ty : In oI = unit;
-    oF : No;
-    oF_ty : Out oF = unit;
+    Mo : choiceType; (* Oracle memories. *)
+    No : choiceType; (* Oracle names. *)
+    In : No -> choiceType; (* Oracle input types. *)
+    Out : No -> choiceType; (* Oracle output types. *)
+    Oo : (* Oracle implementation. *)
+      forall (o : No), In o -> Mo -> itree Rnd (Out o * Mo);
+    orac_init_mem : Mo; (* Initial oracle memory. *)
   }.
 
 Context {O : OracleSystem}.
 
-Definition Res := In oF.
+(* An exchange: the name of an oracle, an input to that oracle, and the output
+   returned by that oracle. *)
+Definition Xch := { o : No & (In o * Out o)%type }.
 
-Definition Xch := { o : No & In o & Out o }.
+(* A trace is a sequence of exchanges and intermediate memories. *)
 Definition trace := seq (Mo * Xch).
 
+(* Exchange event that the adversary triggers. *)
 Variant Exch : Type -> Type :=
   Exchange : forall o : No, In o -> Exch (Out o).
 
 Class Adversary :=
   {
-    Ma : choiceType;
-    adv_init_mem : Ma;
-    adv_run : Ma -> itree Exch Ma;
+    Ma : choiceType; (* Adversary's memory. *)
+    Aa : itree Exch Ma; (* Adversary's algorithm. *)
   }.
 
 Context {A : Adversary}.
@@ -87,8 +89,8 @@ Context {A : Adversary}.
 Definition get_Mo E `{stateE trace -< E} : itree E Mo :=
   let* t := get in Ret (head orac_init_mem [seq fst x | x <- t ]).
 
-Definition mk (m : Mo) (o : No) (i : In o) (r : Out o) :=
-  (m, existT2 In Out o i r).
+Definition mk {o : No} (m : Mo) (i : In o) (r : Out o) : Mo * Xch :=
+  (m, existT (fun _ => _)%type o (i, r)).
 
 Definition log E `{stateE trace -< E}
   (m : Mo) (o : No) (i : In o) (r : Out o) : itree E unit :=
@@ -102,18 +104,136 @@ Definition handle_Exch : Exch ~> itree (stateE trace +' Rnd) :=
     let* _ := log m' i r in
     Ret r.
 
-Definition composition (E : trace -> Ma -> bool) : itree Rnd bool :=
-  let c := interp handle_Exch (adv_run adv_init_mem) in
-  let* (t, m) := run_state c [::] in
-  Ret (E t m).
+Definition interact : itree Rnd (trace * Ma) :=
+  run_state (interp handle_Exch Aa) [::].
+
+Definition dinteract : distr (trace * Ma)%type := dinterp interact.
+
+Class WinningCondition :=
+  {
+    win : trace -> Ma -> bool;
+  }.
+
+Context {W : WinningCondition}.
+
+Definition pwin : R := \P_[ dinteract ] (fun p => win p.1 p.2).
 
 End CIL.
 
-Notation "\Pr_[ A | O | E ]" :=
-  (\P_[ dinterp (composition (A := A) (O := O) E) ] id).
-
-Context {O : OracleSystem} {A : Adversary}.
-
-Check \Pr_[ A | O | fun _ _ => true ] : R.
-
 End MAIN.
+
+Arguments pwin {_} _ _ _.
+
+Require indcca.
+
+Section INSTANCE.
+
+Context
+  {R : realType}
+  {pkey skey advmem : choiceType}
+  {ciphert : choiceType}
+  {msg : finType}
+  {dummy : msg}
+  {C : @indcca.Challenger R pkey skey ciphert msg}
+  {A : @indcca.Adversary R pkey advmem ciphert msg}
+  {Q : nat}
+.
+
+Notation distr := (distr R).
+Notation Rnd := (Rnd (R := R)).
+Notation OracleSystem := (OracleSystem (R := R)).
+Notation Adversary := (Adversary (R := R)).
+Notation WinningCondition := (WinningCondition (R := R)).
+
+Definition advantage := indcca.advantage (dummy := dummy) C A Q.
+Definition game := indcca.game (dummy := dummy) C A Q.
+
+Definition _Mo := option (skey * msg).
+
+Definition _No := option bool. (* finType doesn't work with a variant... *)
+
+Notation "'GenKey'" := (None) (at level 0, only parsing).
+Notation "'Encap'" := (Some true) (at level 0, only parsing).
+Notation "'Decap'" := (Some false) (at level 0, only parsing).
+
+Definition _In (x : _No) : choiceType :=
+  match x with
+  | GenKey => unit
+  | Encap => pkey
+  | Decap => ciphert
+  end.
+
+Definition _Out (x : _No) : choiceType :=
+  match x with
+  | GenKey => pkey
+  | Encap => ciphert
+  | Decap => msg
+  end.
+
+Definition _Oo (x : _No) : _In x -> _Mo -> itree Rnd (_Out x * _Mo) :=
+  match x return _In x -> _Mo -> itree Rnd (_Out x * _Mo) with
+  | GenKey =>
+      fun _ _ =>
+        let* (pk, sk) := C.(indcca.GenKey) in
+        Ret (pk, Some (sk, dummy))
+  | Encap =>
+      fun pk s =>
+        let* (ct, m) := C.(indcca.Encap) pk in
+        if s is Some (sk, _) then Ret (ct, Some (sk, m))
+        else Ret (ct, None)
+  | Decap =>
+      fun ct s =>
+        if s is Some (sk, _) then
+          let* m := C.(indcca.Decap) sk ct in
+          Ret (m, s)
+        else Ret (dummy, None)
+  end.
+
+Instance INDCCA : OracleSystem :=
+  {|
+    Mo := _Mo;
+    No := _No;
+    In := _In;
+    Out := _Out;
+    Oo := _Oo;
+    orac_init_mem := None;
+  |}.
+
+Context {A' : Adversary}.
+
+Instance W : WinningCondition. Admitted. (* ?? *)
+
+Definition interact_aux : itree Rnd bool :=
+  let* (t, m) := interact in Ret (win t m).
+
+Lemma pr_dlet_id T (mu : distr.distr R T) E :
+  \P_[mu] E = \P_[ \dlet_(x <- mu) dunit (E x) ] id.
+Proof. by rewrite -dmarginE pr_dmargin. Qed.
+
+Lemma dinterp_bind (T1 T2 : choiceType) (t : itree Rnd T1) (k : T1 -> itree Rnd T2) :
+  dinterp (let* x := t in k x) = \dlet_(x <- dinterp t) dinterp (k x).
+Admitted.
+
+Lemma dinterp_Ret (T : choiceType) (r : T) :
+  dinterp (R := R) (Ret r) =1 dunit r.
+Proof.
+move=> x; rewrite -dlim_bump (eq_dlim (g := fun=> dunit r)) //; exact/dlimC.
+Qed.
+
+Lemma interact_auxP : pwin INDCCA A' W = \P_[ dinterp interact_aux ] id.
+Proof.
+rewrite /pwin/interact_aux pr_dlet_id; apply/eq_mu_pr => x.
+rewrite dinterp_bind; apply/eq_in_dlet; last done.
+move=> [t m] _ b; by rewrite dinterp_Ret.
+Qed.
+
+Lemma eutt_interact_game : eutt eq interact_aux game.
+Admitted.
+
+Lemma correct_indcca : `| pwin INDCCA A' W - 1/2 | = advantage.
+Proof.
+rewrite interact_auxP /advantage /indcca.advantage; do 2!f_equal.
+exact/eq_mu_pr/dinterp_eutt/eutt_interact_game.
+Qed.
+
+End INSTANCE.
